Prove an `assume`

fstar/MLS.MiscLemmas.fst
@@ -1,5 +1,9 @@
 module MLS.MiscLemmas
 
+open Comparse
+
+#push-options "--fuel 1 --ifuel 1"
+
 val list_for_all_eq: #a:eqtype -> p:(a -> bool) -> l:list a -> Lemma
   (List.Tot.for_all p l <==> (forall x. List.Tot.mem x l ==> p x))
 let rec list_for_all_eq #a p l =
@@ -13,3 +17,12 @@ let rec mem_filter #a p l x =
   match l with
   | [] -> ()
   | h::t -> mem_filter p t x
+
+#push-options "--fuel 2"
+val bytes_length_unsnoc: #bytes:Type0 -> {|bytes_like bytes|} -> #a:Type -> ps_a:parser_serializer_unit bytes a -> l:list a{List.Tot.length l > 0} -> Lemma
+  (let (tl, hd) = List.Tot.unsnoc l in bytes_length ps_a l == bytes_length ps_a tl + (prefixes_length (ps_a.serialize hd)))
+let rec bytes_length_unsnoc #bytes #bl #a ps_a l =
+  match l with
+  | [x] -> ()
+  | h::t -> bytes_length_unsnoc ps_a t
+#pop-options
